@prefix : <https://schema.org/> .
@prefix rdf: <http://www.w3.org/1999/02/22-rdf-syntax-ns#> .
@prefix rdfs: <http://www.w3.org/2000/01/rdf-schema#> .
@prefix xml: <http://www.w3.org/XML/1998/namespace> .
@prefix xsd: <http://www.w3.org/2001/XMLSchema#> .

:MemberProgram a rdfs:Class ;
	rdfs:label "MemberProgram" ;
    :isPartOf <https://pending.schema.org> ;
    :source <https://github.com/schemaorg/schemaorg/issues/3563> ;	
    rdfs:comment "A MemberProgram defines a loyalty (or membership) program that provides its members with certain benefits, for example better pricing, free shipping or returns, or the ability to earn membership points. Member programs typically have different tiers, for example silver and gold members, each with different benefits." ;
    rdfs:subClassOf :Intangible .
	
:MemberProgramTier a rdfs:Class ;
	rdfs:label "MemberProgramTier" ;
    :isPartOf <https://pending.schema.org> ;
    :source <https://github.com/schemaorg/schemaorg/issues/3563> ;	
    rdfs:comment "A MemberProgramTier specifies a tier under a loyalty (member) program, for example \"gold\"." ;
    rdfs:subClassOf :Intangible .

:hasMemberProgram a rdf:Property ;
    rdfs:label "hasMemberProgram" ;
    :domainIncludes :Organization ;
    :rangeIncludes :MemberProgram ;
    :source <https://github.com/schemaorg/schemaorg/issues/3563> ;
    rdfs:comment "MemberProgram offered by an Organization, for example an eCommerce merchant or an airline." .

:forMemberProgram a rdf:Property ;
    rdfs:label "forMemberProgram" ;
    :domainIncludes :MemberProgramTier ;
    :rangeIncludes :MemberProgram ;
    :source <https://github.com/schemaorg/schemaorg/issues/3563> ;
    rdfs:comment "The member program this tier belongs to." .

:hasTiers a rdf:Property ;
    rdfs:label "hasTiers" ;
    :domainIncludes :MemberProgram ;
    :rangeIncludes :MemberProgramTier ;
    :source <https://github.com/schemaorg/schemaorg/issues/3563> ;
    rdfs:comment "The tiers of a member program." .


:TierRequirementEnumeration a rdfs:Class ;
	rdfs:label "TierRequirementEnumeration" ;
	:isPartOf <https://pending.schema.org> ;
	:source <https://github.com/schemaorg/schemaorg/issues/3563> ;
	rdfs:comment "An enumeration of requirements to join a tier in a membership program." ;
	rdfs:subClassOf :Enumeration .
	
:TierFreeToJoin a :TierRequirementEnumeration ;
    rdfs:label "TierFreeToJoin" ;
    :isPartOf <https://pending.schema.org> ;
    :source <https://github.com/schemaorg/schemaorg/issues/3563> ;
    rdfs:comment "Membership tier is free to join." .
	
:TierSpendingAmountRequired a :TierRequirementEnumeration ;
    rdfs:label "TierSpendingAmountRequired" ;
    :isPartOf <https://pending.schema.org> ;
    :source <https://github.com/schemaorg/schemaorg/issues/3563> ;
    rdfs:comment "Membership tier requires a minimum amount of spending." .

:TierCreditCardRequired a :TierRequirementEnumeration ;
    rdfs:label "TierCreditCardRequired" ;
    :isPartOf <https://pending.schema.org> ;
    :source <https://github.com/schemaorg/schemaorg/issues/3563> ;
    rdfs:comment "Membership tier requires sign up for a credit card." .

:TierPeriodicFeeRequired a :TierRequirementEnumeration ;
    rdfs:label "TierPeriodicFeeRequired" ;
    :isPartOf <https://pending.schema.org> ;
    :source <https://github.com/schemaorg/schemaorg/issues/3563> ;
    rdfs:comment "Membership tier requires payment of a periodic fee." .

:hasTierRequirement a rdf:Property ;
    rdfs:label "hasTierRequirement" ;
    :domainIncludes :MemberProgramTier ;
    :rangeIncludes :TierRequirementEnumeration,
		 :Text;
    :source <https://github.com/schemaorg/schemaorg/issues/3563> ;
    rdfs:comment "A requirement to join a tier of a membership program." .

:hasTierBenefit a rdf:Property ;
    rdfs:label "hasTierBenefit" ;
    :domainIncludes :MemberProgramTier ;
    :rangeIncludes :TierBenefitEnumeration,
		 :Text;
    :source <https://github.com/schemaorg/schemaorg/issues/3563> ;
    rdfs:comment "A member benefit for a tier of a membership program." .


:minimumSpendingAmount a rdf:Property ;
    rdfs:label "minimumSpendingAmount" ;
    :domainIncludes :MemberProgramTier ;
    :rangeIncludes :MonetaryAmount ;
    :source <https://github.com/schemaorg/schemaorg/issues/3563> ;
    rdfs:comment "The minimum amount of spending required to join a membership tier, corresponding to enumeration value [TierSpendingAmountRequired](https://schema.org/TierSpendingAmountRequired)." .
	
:creditCard a rdf:Property ;
    rdfs:label "creditCard" ;
    :domainIncludes :MemberProgramTier ;
    :rangeIncludes :Text ;
    :source <https://github.com/schemaorg/schemaorg/issues/3563> ;
    rdfs:comment "Description of the credit card required to join a membership tier, corresponding to enumeration value [TierCreditCardRequired](https://schema.org/TierCreditCardRequired)." .

:periodicFee a rdf:Property ;
    rdfs:label "periodicFee" ;
    :domainIncludes :MemberProgramTier ;
    :rangeIncludes :MonetaryAmount ;
    :source <https://github.com/schemaorg/schemaorg/issues/3563> ;
    rdfs:comment "The periodic fee required to join a membership tier, corresponding to enumeration value [TierPeriodicFeeRequired](https://schema.org/TierPeriodicFeeRequired). Use in combination with [periodLength](https://schema.org/periodLength)." .

:periodLength a rdf:Property ;
    rdfs:label "periodLength" ;
    :domainIncludes :MemberProgramTier ;
    :rangeIncludes :QuantitativeValue ;
    :source <https://github.com/schemaorg/schemaorg/issues/3563> ;
    rdfs:comment "How long a member is part of a membership tier after paying the periodic membership fee, corresponding to enumeration value [TierPeriodicFeeRequired](https://schema.org/TierPeriodicFeeRequired). Use in combination with [periodicFee](https://schema.org/periodicFee)." .



:TierBenefitEnumeration a rdfs:Class ;
	rdfs:label "TierBenefitEnumeration" ;
	:isPartOf <https://pending.schema.org> ;
	:source <https://github.com/schemaorg/schemaorg/issues/3563> ;
	rdfs:comment "An enumeration of possible benefits as part of a loyalty (members) program." ;
	rdfs:subClassOf :Enumeration .
	
:TierBenefitLoyaltyPrice a :TierBenefitEnumeration ;
    rdfs:label "TierBenefitLoyaltyPrice" ;
    :isPartOf <https://pending.schema.org> ;
    :source <https://github.com/schemaorg/schemaorg/issues/3563> ;
    rdfs:comment "Benefit of the tier is a members-only price." .

:TierBenefitLoyaltyShipping a :TierBenefitEnumeration ;
    rdfs:label "TierBenefitLoyaltyShipping" ;
    :isPartOf <https://pending.schema.org> ;
    :source <https://github.com/schemaorg/schemaorg/issues/3563> ;
    rdfs:comment "Benefit of the tier is a members-only shipping price or speed (for example free shipping or 1-day shipping)." .

:TierBenefitLoyaltyReturns a :TierBenefitEnumeration ;
    rdfs:label "TierBenefitLoyaltyReturns" ;
    :isPartOf <https://pending.schema.org> ;
    :source <https://github.com/schemaorg/schemaorg/issues/3563> ;
    rdfs:comment "Benefit of the tier is members-only returns, for example free unlimited returns." .

:TierBenefitLoyaltyPoints a :TierBenefitEnumeration ;
    rdfs:label "TierBenefitLoyaltyPoints" ;
    :isPartOf <https://pending.schema.org> ;
    :source <https://github.com/schemaorg/schemaorg/issues/3563> ;
    rdfs:comment "Benefit of the tier is earning of loyalty points." .

:MemberPrice a :PriceTypeEnumeration ;
    rdfs:label "MemberPrice" ;
    :isPartOf <https://pending.schema.org> ;
    :source <https://github.com/schemaorg/schemaorg/issues/3563> ;
    rdfs:comment "Indicates the price is for members of a loyalty program only." .

:validForMemberTier a rdf:Property ;
    rdfs:label "validForMemberTier" ;
    :domainIncludes :Offer,
		 :PriceSpecification,
		 :OfferShippingDetails,
		 :MerchantReturnPolicy;
    :rangeIncludes :MemberProgramTier ;
    :source <https://github.com/schemaorg/schemaorg/issues/3563> ;
    rdfs:comment "The membership program tier an Offer (or a PriceSpecification, OfferShippingDetails, or MerchantReturnPolicy under an Offer) is valid for." .

:membershipPointsEarned a rdf:Property ;
    :domainIncludes :MemberProgramTier, 
		:PriceSpecification .

